\input{../include/preamble}

\title[ID1019 Interpreter]{The Interpreter}


\author{Johan Montelius}
\institute{KTH}
\date{\semester}

\begin{document}

\begin{frame}
\titlepage
\end{frame}


\begin{frame}{the language}
  
\begin{grammar}
<atom> ::= :a | :b | :c | \ldots

<variable> ::= x | y | z | \ldots

<literal> ::= <atom>

<expression> ::= <literal> | <variable> |  '\{' <expression> ',' <expression> '\}'

<pattern> ::= <literal> 
      \alt <variable> 
      \alt '\_' 
      \alt '\{' <pattern> ',' <pattern> '\}'

<match> ::=  <pattern> '=' <expression>

<sequence> ::=  <expression> \alt <match> ';' <sequence>
\end{grammar}

\end{frame} 

\begin{frame}{the domain}


$${\rm Atoms} =  \{a,b,c, ...\}$$

$${\rm Structures} = {\rm Atoms} \cup \{\{s_1, s_2\} | s_i \in {\rm Structures}\}$$

\end{frame}


\begin{frame}{operational semantics}

\vspace{10pt}
$$\frac{{\rm prerequisite}}{E\sigma({\rm expression}) \rightarrow {\rm result}}$$

\vspace{20pt}

\begin{itemize}
\item Evaluation of expressions: $E\; {\rm env}\; ({\rm expr}) \; \rightarrow \; \perp \; \cup \; {\rm Structures}$
\item Pattern matching: $P\; {\rm env}\; ({\rm pattern}, \; {\rm struct})\;  \rightarrow \; {\rm fail} \; \cup\;  {\rm Environments}$
\end{itemize}

\vspace{40pt}{\em This is called ``big step'' operational semantics.''}

\end{frame}


\begin{frame}{evaluation of expressions}


$$\frac{a \equiv s}{E\sigma(a) \rightarrow s}$$

$$\frac{v/s \in \sigma}{E\sigma(v) \rightarrow s}$$

$$\frac{ E\sigma(e_1) \rightarrow s_1 \qquad   E\sigma(e_2) \rightarrow s_2}{E\sigma(\lbrace e_1 , e_2\rbrace) \rightarrow \{s_1, s_2\}}$$

$$\frac{ v/s \not\in \sigma}{E\sigma(v) \rightarrow  \perp}$$

\end{frame}


\begin{frame}{pattern matching}


$$\frac{a \equiv s}{P\sigma(a, s) \rightarrow \sigma}$$ 

$$\frac{v/t \not\in \sigma}{P\sigma(v, s) \rightarrow \lbrace v/s \rbrace \cup \sigma}$$

$$\frac{v/s \in \sigma}{P\sigma(v, s) \rightarrow \sigma}$$ 

$$\frac{}{P\sigma(\_, s) \rightarrow \sigma}$$ 

$$\frac{a \not\equiv s}{P\sigma(a, s) \rightarrow {\rm fail}}$$ 

$$\frac{v/t \in \sigma \qquad  t \not\equiv s}{P\sigma(v, s) \rightarrow {\rm fail}}$$ 

\end{frame}

\begin{frame}{pattern matching}


$$\frac{P\sigma(p_1, s_1) \rightarrow \sigma' \wedge P\sigma'(p_2, s_2) \rightarrow \theta}{P\sigma(\lbrace p_1, p_2 \rbrace  , \lbrace s_1, s_2 \rbrace) \rightarrow \theta}$$

\vspace{10pt}
$$\frac{P\sigma(p_1, s_1) \rightarrow {\rm fail} }{P\sigma(\lbrace p_1, p_2 \rbrace  , \lbrace s_1, s_2 \rbrace) \rightarrow {\rm fail}}$$

\vspace{10pt}
$$\frac{P\sigma(p_1, s_1) \rightarrow \sigma' \wedge P\sigma'(p_2, s_2) \rightarrow {\rm fail}}{P\sigma(\lbrace p_1, p_2 \rbrace  , \lbrace s_1, s_2 \rbrace) \rightarrow {\rm fail}}$$


\vspace{40pt}{\em Match a compund pattern with anyting but a compound structure will fail.}

\end{frame}


\begin{frame}{evaluation of sequences}


$$\frac{\sigma' = \sigma \setminus \lbrace v/t \quad | \quad v/t \in \sigma \quad \wedge \quad  v \quad {\rm in} \quad p\rbrace}{S(\sigma, p) \rightarrow \sigma'}$$
  

$$\frac{   
  E\sigma(e) \rightarrow t
  \qquad S(\sigma, p) \rightarrow \sigma' 
  \qquad P\sigma'(p, t) \rightarrow \theta
  \qquad E\theta({\rm sequence}) \rightarrow s
}{E\sigma(p = e; {\rm sequence}) \rightarrow s}$$ 


\end{frame}


\begin{frame}{case expression}

\begin{grammar}
     <expression> ::=  <case expression> | ...  

     <case expression> ::= 'case' <expression> 'do' <clauses>  'end' 

     <clauses> ::=   <clause> | <clause> ';' <clauses>

     <clause> ::=  <pattern> '->' <sequence>
\end{grammar}
\end{frame}

\begin{frame}{evaluation of case expression}


$$\frac{E\sigma(e) \rightarrow t \qquad C\sigma(t, {\rm clauses}) \rightarrow s }{E\sigma({\tt case}\ e \ {\tt do}\ {\rm clauses} \ {\tt end}) \rightarrow s}$$
  
\end{frame}
\begin{frame}{selection of a clause}

$$\frac{
  S(\sigma, p) \rightarrow \sigma' \qquad
  P\sigma'(p, s) \rightarrow \theta \qquad
  \theta \not = {\rm fail} \qquad
  E\theta({\rm sequence}) \rightarrow s}{
C\sigma(s, p \;{\rm ->}\;    {\rm sequence} ; {\rm clauses}) \rightarrow s}$$

\vspace{10pt}

$$\frac{
  S(\sigma, p) \rightarrow \sigma'   \qquad
  P\sigma'(p, s) \rightarrow {\rm fail} \qquad
  C\sigma(s, {\rm clauses}) \rightarrow s}{
C\sigma(s, p \;{\rm -\textgreater}\;  {\rm sequence} ; {\rm clauses}) \rightarrow s}$$

\vspace{10pt}

$$\frac{
  S(\sigma, p) \rightarrow \sigma' \qquad
  P\sigma'(p, s) \rightarrow {\rm fail} }{
C\sigma(s, p \;{\rm -\textgreater}\;  {\rm sequence}) \rightarrow \perp}$$


\end{frame}





\begin{frame}[fragile]{variable scope}

\vspace{20pt}

\hspace{20pt}
\begin{verbatim}
   y = case :a do
         :a -> z = 42, {:b, z}
       end;
   {y, z}
\end{verbatim}

\vspace{20pt}{\em This is not allowed in our language, \texttt{Z} in
  \texttt{\{Y,Z\}} is a free variable. However .... \pause this is
  allowed in Elixir and Erlang (but it should not be).}

\end{frame}
 
\begin{frame}{what's missing}

\vspace{20pt}\hspace{20pt} Handle lambda expressions, closures and function application.
  
\end{frame}


\begin{frame}[fragile]{lambda expressions}

  \vspace{20pt}

  \begin{tabular}{r l l}
   {\em Atoms} & = & \{a, b, c, \ldots\} \\
   {\em Closures} & = & \{<p:s:e> | p $\in $ Parameters $\wedge$ s $\in $ Sequence $\wedge$  e $\in $ Environment \}\\
   {\em Structures} & = & {\em Closures} $\cup$ {\em Atoms} $\cup$ \{ \{a, b\} \textbar a $\in$ {\em Structures}  $\wedge$  b $\in$ {\em Structures} \}
  \end{tabular}



\end{frame}

\begin{frame}[fragile]{syntax for function expressions}

\begin{grammar}
  <function> ::= 'fn' '(' <parameters> ')' '->' <sequence> 'end'
  
   <parameters> ::= '  ' | <variables> 

   <variables> ::= <variable> |  <variable> ',' <variables>

   <application> ::= <expression> '.(' <arguments> ')'

   <arguments> ::= '  ' | <expressions>
   
   <expressions> ::= <expression> |  <expression> ',' <expressions>

   <expression> ::= <function> | <application> | ...
\end{grammar}

\end{frame}

\begin{frame}[fragile]{evaluation of a function expression}

$$\frac{ \theta = \{ v/s \mid  v/s \in \sigma \wedge v {\rm\ free\  in\ sequence}\}}{
E\sigma(\texttt{fn (} {\rm parameters}\;  \texttt{) ->}\; {\rm sequence}\; \texttt{end} ) \rightarrow \quad \langle{\rm parameters}:{\rm sequence}:\theta\rangle}$$

\end{frame}


\begin{frame}[fragile]{evaluation of a function application}

$$\frac{E\sigma(e) \rightarrow <v_1, \ldots:{\rm seq}:\theta > \qquad E\sigma(e_i) \rightarrow s_i \qquad E\{v_1/s_1, \ldots\}\cup\theta({\rm seq}) \rightarrow s}{
E\sigma(e.(e_1, \ldots)) \rightarrow s}$$ 


\end{frame}




\end{document}
